consistentcy almost works

src/FcEtt/ext_consist.v
@@ -29,11 +29,10 @@ Export red.
 Set Implicit Arguments.
 Set Bullet Behavior "Strict Subproofs".
 
-
 Definition Good (G : context) (D : available_props):=
   erased_context G /\
-  forall c1 A B1 T1,
-    binds c1 (Co (Eq A B1 T1)) G
+  forall c1 A B1 T1 R,
+    binds c1 (Co (Eq A B1 T1 R)) G
     -> c1 `in` D
     -> exists C, Par G D A C /\ Par G D B1 C.
 
@@ -55,9 +54,9 @@ Proof.
 Qed.
 
 
-Lemma a_Pi_head : forall S G b A rho B,
-    Par S G (a_Pi rho A B) b -> exists A' B' L,
-      b = a_Pi rho A' B' /\ Par S G A A' /\
+Lemma a_Pi_head : forall S G b A R rho B,
+    Par S G (a_Pi rho A R B) b -> exists A' B' L,
+      b = a_Pi rho A' R B' /\ Par S G A A' /\
       (forall x, x `notin` L -> Par S G (open_tm_wrt_tm B (a_Var_f x)) (open_tm_wrt_tm B' (a_Var_f x))).
 Proof.
   intros. inversion H. subst. inversion H0.  exists A , B, empty. split; auto.
@@ -420,7 +419,7 @@ Proof.
     pick fresh x.
     use_size_induction A ac Par1 Par2.
     use_size_induction_open B x bc Par3 Par4.
-    exists (a_Pi rho ac (close_tm_wrt_tm x bc)).
+    exists (a_Pi rho ac R (close_tm_wrt_tm x bc)).
     split; eauto; try solve [apply (@Par_Pi_exists x); eauto].
   - (* cabs cong / cabs cong *)
     pick fresh c.
@@ -433,10 +432,10 @@ Proof.
     use_size_induction A1 AC1 Par5 Par6.
     pick fresh c.
     use_size_induction_open a0 c ac Par7 Par8.
-    exists (a_CPi (Eq AC BC AC1) (close_tm_wrt_co c ac)).
+    exists (a_CPi (Eq AC BC AC1 R) (close_tm_wrt_co c ac)).
     split; eauto; try solve [apply (@Par_CPi_exists c); eauto].
   - (* fam / fam *)
-    have E: (Ax a1 A = Ax a2 A0). eapply binds_unique; eauto using uniq_toplevel.
+    have E: (Ax a1 A R = Ax a2 A0 R0). eapply binds_unique; eauto using uniq_toplevel.
     inversion E. subst. clear E.
     have LC: lc_tm a2. apply Toplevel_lc in H. inversion H. auto.
     exists a2. split; eauto.
@@ -467,8 +466,8 @@ Qed.
 
 Ltac binds_notbinds :=
     match goal with
-    [ H0 : binds ?c (Ax ?T ?a) toplevel,
-      H5 : forall (c : atom) a, not (binds c (Ax ?T a) an_toplevel) |- _  ] =>
+    [ H0 : binds ?c (Ax ?T ?a ?R) toplevel,
+      H5 : forall (c : atom) a, not (binds c (Ax ?T a ?R) an_toplevel) |- _  ] =>
       unfold not in H5; unfold toplevel in H0; unfold erase_sig in H0;
       apply binds_map_3 in H0; destruct H0 as (s' & EQ & B);
       destruct s'; simpl in EQ; inversion EQ; subst;
@@ -490,20 +489,20 @@ Proof.
 Qed.
 
 
-Lemma multipar_Pi : forall S D rho A B, multipar S D A B -> forall A1 A2,
-      A = a_Pi rho A1 A2 -> exists B1 B2, B = (a_Pi rho B1 B2).
-intros S D rho A B H. induction H. intros. subst. exists A1, A2. auto.
+Lemma multipar_Pi : forall S D rho R A B, multipar S D A B -> forall A1 A2,
+      A = a_Pi rho A1 R A2 -> exists B1 B2, B = (a_Pi rho B1 R B2).
+intros S D rho A R B H. induction H. intros. subst. exists A1, A2. auto.
 intros. subst.
 inversion H; subst; destruct (IHmultipar _ _ eq_refl) as [B1 [B2 EQ]]; auto;
 exists B1, B2; auto.
 Qed.
 
-Lemma multipar_CPi : forall S D A C, multipar S D A C -> forall A1 A2 A3 B, A = a_CPi (Eq A1 A2 A3) B -> exists B1 B2 B3 C2,
-        C = (a_CPi (Eq B1 B2 B3) C2).
+Lemma multipar_CPi : forall S D A C, multipar S D A C -> forall A1 A2 A3 R B, A = a_CPi (Eq A1 A2 A3 R) B -> exists B1 B2 B3 C2,
+        C = (a_CPi (Eq B1 B2 B3 R) C2).
 Proof.
   intros S D A C H. induction H; intros; subst.
   exists A1, A2, A3, B. auto.
-  inversion H; subst; destruct (IHmultipar _ _ _ _ eq_refl) as [B1 [B2 [C2 EQ]]];
+  inversion H; subst; destruct (IHmultipar _ _ _ _ _ eq_refl) as [B1 [B2 [C2 EQ]]];
     auto; exists B1, B2, C2; auto.
 Qed.
 
@@ -529,12 +528,12 @@ Qed.
 
 
 
-Lemma multipar_CAbs : forall S D A C, multipar S D A C -> forall A1 A2 A3 B, A = a_CAbs (Eq A1 A2 A3) B -> exists B1 B2 B3 C2,
-        C = (a_CAbs (Eq B1 B2 B3) C2).
+Lemma multipar_CAbs : forall S D A C, multipar S D A C -> forall A1 A2 A3 R B, A = a_CAbs (Eq A1 A2 A3 R) B -> exists B1 B2 B3 C2,
+        C = (a_CAbs (Eq B1 B2 B3 R) C2).
 Proof.
   intros S D A C H. induction H; intros; subst.
   exists A1, A2, A3, B. auto.
-  inversion H; subst; destruct (IHmultipar _ _ _ _ eq_refl) as [B1 [B2 [C2 EQ]]];
+  inversion H; subst; destruct (IHmultipar _ _ _ _ _ eq_refl) as [B1 [B2 [C2 EQ]]];
     auto; exists B1, B2, C2; auto.
 Qed.
 
@@ -553,7 +552,7 @@ Ltac multipar_step SIDE EQ :=
   match goal with
   | [ SIDE : multipar _ _ a_Star _ |- _ ] =>
     apply multipar_Star in SIDE; auto; rename SIDE into EQ
-  | [ SIDE : multipar _ _ (a_Pi _ _ _) _ |- _ ] =>
+  | [ SIDE : multipar _ _ (a_Pi _ _ _ _) _ |- _ ] =>
     destruct (multipar_Pi SIDE eq_refl) as [b1' [b2' EQ]]
   | [ SIDE : multipar _ _ (a_CPi ?phi _) _ |- _ ] =>
     try (destruct phi); destruct (multipar_CPi SIDE eq_refl)
@@ -749,10 +748,10 @@ Hint Resolve Good_NoAssn.
 
 Hint Resolve multipar_context_independent.
 
-Lemma Good_add_tm: forall G D x A,
-    erased_tm A -> Good G D -> Good ((x, Tm A)::G ) D.
+Lemma Good_add_tm: forall G D x A R,
+    erased_tm A -> Good G D -> Good ((x, Tm A R)::G ) D.
 Proof.
-  intros G D x A E H.
+  intros G D x A R E H.
   unfold Good in *.
   split.
   + unfold erased_context in *.
@@ -763,7 +762,7 @@ Proof.
     - split_hyp.
       eapply Forall_forall in H; eauto.
       simpl in H. auto.
-  + intros c1 A1 B1 T1 BI1 I1.
+  + intros c1 A1 B1 T1 R0 BI1 I1.
   destruct H as (Es & M).
   apply binds_cons_1 in BI1.
   destruct BI1 as [[_ EQ] | BI1]. inversion EQ.
@@ -775,9 +774,9 @@ Proof.
     apply binds_cons; auto.
 Qed.
 
-Lemma Good_add_tm_2: forall G D x A, x `notin` dom G -> erased_tm A -> Good G D -> Good ((x, Tm A)::G ) (add x D).
+Lemma Good_add_tm_2: forall G D x A R, x `notin` dom G -> erased_tm A -> Good G D -> Good ((x, Tm A R)::G ) (add x D).
 Proof.
-  intros G D x A FR E H.
+  intros G D x A R FR E H.
   unfold Good in *.
   split.
   + unfold erased_context in *.
@@ -788,7 +787,7 @@ Proof.
     - split_hyp.
       eapply Forall_forall in H; eauto.
       simpl in H. auto.
-  + intros c1 A1 B1 T1 BI1 I1.
+  + intros c1 A1 B1 T1 R0 BI1 I1.
   destruct H as (Es & M).
   apply binds_cons_1 in BI1.
   destruct BI1 as [[_ EQ] | BI1]. inversion EQ.
@@ -1006,21 +1005,21 @@ Ltac multipar_CPi c :=
 
 
 Lemma consistent_mutual:
-  (forall S a A,   Typing S a A -> True) /\
+  (forall S a A R,   Typing S a A R -> True) /\
   (forall S phi,   PropWff S phi -> True) /\
-  (forall S D p1 p2, Iso S D p1 p2 -> Good S D -> (forall A1 B1 T1 A2 B2 T2, p1 = Eq A1 B1 T1 -> p2 = Eq A2 B2 T2-> (joins S D A1 A2 /\ joins S D B1 B2 /\ joins S D T1 T2))) /\
-  (forall S D A B T,   DefEq S D A B T -> Good S D -> joins S D A B) /\
+  (forall S D p1 p2, Iso S D p1 p2 -> Good S D -> (forall A1 B1 T1 A2 B2 T2 R1 R2, p1 = Eq A1 B1 T1 R1 -> p2 = Eq A2 B2 T2 R2 -> (joins S D A1 A2 /\ joins S D B1 B2 /\ joins S D T1 T2))) /\
+  (forall S D A B T R,   DefEq S D A B T R -> Good S D -> joins S D A B) /\
   (forall S,       Ctx S -> True).
 Proof.
   apply typing_wff_iso_defeq_mutual; eauto; try done.
-  - intros G D A1 B1 A A2 B2 d H d0 H0 H1 A0 B0 T1 A3 B3 T2 H2 H3.
+  - intros G D A1 B1 A R A2 B2 d H d0 H0 H1 A0 B0 T1 A3 B3 T2 R1 R2 H2 H3.
     inversion H2; subst; clear H2.
     inversion H3; subst; clear H3.
     repeat split; eauto.
     exists T2; eauto.
     have et: erased_tm T2.
     apply DefEq_regularity in d.
-    pose K := (second typing_erased_mutual) _ _ d A0 A3 T2.
+    pose K := (second typing_erased_mutual) _ _ d A0 A3 T2 R2.
     apply K; auto.
     repeat split; auto.
     have C: Ctx G by eauto.
@@ -1033,19 +1032,19 @@ Proof.
     destruct phi. apply binds_to_PropWff in H2.
     inversion H2.
     eapply erased_Co; eauto using Typing_erased. auto.
-  - intros G D A1 A2 A B d H p H0 p0 H1 H2 A0 B1 T1 A3 B2 T2 H3 H4.
+  - intros G D A1 A2 A R B d H p H0 p0 H1 H2 A0 B1 T1 A3 B2 T2 R1 R2 H3 H4.
     inversion H4; subst; clear H4.
     inversion H3; subst; clear H3.
     inversion p; subst.
     inversion H2.
     have lc1: lc_tm A0 by eapply Typing_lc in H7; split_hyp; eauto.
-    have lc2: lc_tm B1 by eapply Typing_lc in H8; split_hyp; eauto.
+    have lc2: lc_tm B1 by eapply Typing_lc in H9; split_hyp; eauto.
     repeat split; eauto.
     + exists A0.
       repeat split; eauto; try solve [eapply (Typing_erased); eauto]; eauto.
     + exists B1.
       repeat split; eauto; try solve [eapply (Typing_erased); eauto]; eauto.
-  - intros G D5 phi1 phi2 B1 B2 d H H0 A1 B0 T1 A2 B3 T2 H1 H2.
+  - intros G D5 phi1 phi2 B1 B2 R d H H0 A1 B0 T1 A2 B3 T2 R1 R2 H1 H2.
     destruct phi1.
     destruct phi2.
     inversion H1; subst; clear H1.
@@ -1072,7 +1071,7 @@ Proof.
       inversion H1; subst; clear H1.
       repeat split; eauto.
   - (* assn *)
-    intros G D a b A c c0 H b0 i H0.
+    intros G D a b A R c c0 H b0 i H0.
     destruct H0 as (Es & M).
     edestruct (M c); eauto.
     split_hyp.
@@ -1083,13 +1082,13 @@ Proof.
     inversion h1.
     unfold joins. exists x. repeat split; eauto.
   - (* refl *)
-    intros G D a A t H H0.
+    intros G D a A R t H H0.
     inversion H0.
     unfold joins. exists a.
     repeat split; try solve [eapply (Typing_erased); eauto]; eauto.
   - (* symmetry *)
-    intros G D a b A d H H0.
-    unfold joins in *. destruct H as [c [L R]]; auto.
+    intros G D a b A R d H H0.
+    unfold joins in *. destruct H as [c [L R0]]; auto.
     exists c. tauto.
   - (* transitivity *)
     intros. eapply join_transitive; auto.
@@ -1109,24 +1108,24 @@ Proof.
     repeat split; eauto.
     eapply Typing_erased; eauto.
   - (* pi-cong *)
-    intros L G D rho A1 B1 A2 B2 d H d0 H0 _ _ t H1 t0 H2 H3.
+    intros L G D rho A1 R B1 A2 B2 R' d H d0 H0 _ _ t H1 t0 H2 S H3.
     inversion H3.
-    have e0: erased_tm (a_Pi rho A1 B1). eapply Typing_erased; eauto.
+    have e0: erased_tm (a_Pi rho A1 R B1). eapply Typing_erased; eauto.
     inversion e0. subst.
     pose Ih1 := H H3.
     pick fresh x for (L \u (fv_tm_tm_tm B1) \u (fv_tm_tm_tm B2) \u dom G).
-    assert (G' : Good ([(x, Tm A1)] ++ G) D).
+    assert (G' : Good ([(x, Tm A1 R)] ++ G) D).
     { apply Good_add_tm; auto. }
     have: x `notin` L; auto => fr.
     pose Ih2 := H0 x fr G'.
     destruct H as [A'' h1]; auto; subst.
     destruct Ih2 as [B'' h2].
     split_hyp.
-    exists (a_Pi rho A'' (close_tm_wrt_tm x B'')); eauto.
+    exists (a_Pi rho A'' R (close_tm_wrt_tm x B'')); eauto.
     repeat split; eauto 1.
     + apply (@erased_a_Pi L); try solve [apply h2; auto]; try solve [apply h1; auto]; eauto.
       intros x0 h4.
-      assert (G'' : Good ([(x0, Tm A1)] ++ G) D).
+      assert (G'' : Good ([(x0, Tm A1 R)] ++ G) D).
       apply Good_add_tm; auto.
       pose Ih2 := H0 x0 h4 G''.
       destruct Ih2 as [C'' h3]; eauto.
@@ -1138,11 +1137,11 @@ Proof.
       apply (lc_a_Pi_exists x); apply erased_lc; auto.
       eapply multipar_context_independent; eauto.
   - (* abs-cong *)
-    intros L G D rho b1 b2 A1 B IHDefEq H1 t _ RC1 RC2 GOOD.
+    intros L G D rho b1 b2 A1 R B R' IHDefEq H1 t _ S RC1 RC2 GOOD.
     inversion GOOD.
     have e0: erased_tm A1. eapply Typing_erased; eauto.
     pick fresh x for (L \u (fv_tm_tm_tm b1) \u (fv_tm_tm_tm b2)).
-    assert (G' : Good ([(x, Tm A1)] ++ G) D).
+    assert (G' : Good ([(x, Tm A1 R)] ++ G) D).
     apply Good_add_tm; auto.
     have: x `notin` L; auto => fr.
     pose Ih2 := H1 x fr G'.
@@ -1152,14 +1151,14 @@ Proof.
     repeat split; eauto 1.
     + apply (@erased_a_Abs L); try solve [apply h2; auto]; try solve [apply h1; auto]; eauto.
       intros x0 h4.
-      assert (G'' : Good ([(x0, Tm A1)] ++ G) D).
+      assert (G'' : Good ([(x0, Tm A1 R)] ++ G) D).
       apply Good_add_tm; auto.
       pose Ih2 := H1 x0 h4 G''.
       destruct Ih2 as [C'' h3]; eauto.
       apply h3.
     + apply (@erased_a_Abs L); try solve [apply h2; auto]; try solve [apply h1; auto]; eauto.
       intros x0 h4.
-      assert (G'' : Good ([(x0, Tm A1)] ++ G) D).
+      assert (G'' : Good ([(x0, Tm A1 R)] ++ G) D).
       apply Good_add_tm; auto.
       pose Ih2 := H1 x0 h4 G''.
       destruct Ih2 as [C'' h3]; eauto.
@@ -1170,13 +1169,13 @@ Proof.
     + apply multipar_Abs_exists; auto.
       apply (lc_a_UAbs_exists x); apply erased_lc; auto.
       eapply multipar_context_independent; eauto.
-  - intros G D a1 a2 b1 b2 d H d0 H0 p H1 H2.
+  - intros G D a1 a2 b1 b2 d R' H R d0 H0 p H1 H2.
     apply join_app; auto.
-  - intros G D a1 b1 B a A d H t H0 H1.
+  - intros G D a1 b1 B a R' A R d H t H0 H1.
     inversion H1.
     apply join_app; auto.
     exists a_Bullet. repeat split; eauto.
-  - intros G D A1 A2 rho B1 B2 H IHDefEq GOOD.
+  - intros G D A1 A2 R rho B1 B2 R' H IHDefEq GOOD.
     inversion GOOD.
     destruct IHDefEq; auto.
     split_hyp.
@@ -1189,7 +1188,7 @@ Proof.
     exists A'; eauto.
     apply erased_lc; eauto.
     apply erased_lc; eauto.
-  - intros G D B1 a1 B2 a2 rho A1 A2 H IHDefEq1 H0 IHDefEq2 GOOD.
+  - intros G D B1 a1 B2 a2 R' rho A1 R A2 H IHDefEq1 H0 IHDefEq2 GOOD.
     inversion GOOD.
     destruct IHDefEq1; auto.
     destruct IHDefEq2 as [ac h0]; auto.
@@ -1214,15 +1213,15 @@ Proof.
     + multipar_subst_open x.
     + multipar_subst_open x.
   - (* cpi-cong *)
-    intros L G D phi1 A phi2 B H hi0 H1 IHDefEq H2 _ _ t _ _ GOOD .
+    intros L G D phi1 A phi2 B R H hi0 H1 IHDefEq H2 _ _ t _ _ GOOD .
     destruct phi1.
     destruct phi2.
     pick_fresh c.
     match goal with
-      | [ H : Iso G D (Eq a b A0) (Eq a0 b0 A1) |- _ ] =>
-        destruct (hi0 GOOD a b A0 a0 b0 A1) as [hi1 [hi2 hi3]]; auto
+      | [ H : Iso G D (Eq a b A0 R0) (Eq a0 b0 A1 R1) |- _ ] =>
+        destruct (hi0 GOOD a b A0 a0 b0 A1 R0 R1) as [hi1 [hi2 hi3]]; auto
     end.
-    have EC : erased_sort (Co (Eq a b A0)).
+    have EC : erased_sort (Co (Eq a b A0 R0)).
     { inversion H2. apply erased_Co; eapply Typing_erased; eauto. }
     destruct (IHDefEq c) as [Ac h1]; eauto.
     + apply Good_NoAssn; auto.
@@ -1232,7 +1231,7 @@ Proof.
       destruct hi2 as [Bco h1'].
       destruct hi3 as [Tco h2'].
       split_hyp.
-      exists (a_CPi (Eq Aco Bco Tco) (close_tm_wrt_co c Ac)); eauto.
+      exists (a_CPi (Eq Aco Bco Tco R0) (close_tm_wrt_co c Ac)); eauto.
       repeat split; eauto 1.
       * apply (@erased_a_CPi (L \u D)); eauto.
         intros c0 Hi5.
@@ -1245,20 +1244,20 @@ Proof.
         apply Good_NoAssn; auto.
         apply h2'.
       * (* Ltac context_independence c := *)
-(*        eapply multipar_context_independent; eauto.
+     (* eapply multipar_context_independent; eauto.
         intros x; intros; assert (x <> c); [fsetdec|
         match goal with
-          [ H23 : binds ?x (Co (Eq (a_Const ?F) ?a ?A4)) ([(c, Co (Eq ?A0 ?B0 ?A1))] ++ ?G) |- _ ] =>
+          [ H23 : binds ?x (Co (Eq (a_Const ?F) ?a ?A4 ?R)) ([(c, Co (Eq ?A0 ?B0 ?A1 ?R'))] ++ ?G) |- _ ] =>
               simpl in H23;
               edestruct (binds_cons_1 _ x c _ _ G H23) as [[h0 h1] | h2];
               [contradiction| auto]
-        end].   *)
+        end]. *)
         multipar_CPi c.
-      * multipar_CPi c.
-  - intros L G D a b phi1 B hi0 IHDefEq H1 _ GOOD.
+      * admit. (* multipar_CPi c. *)
+  - intros L G D a b phi1 B R hi0 IHDefEq H1 _ GOOD.
     destruct phi1.
     pick_fresh c.
-    have EC : erased_sort (Co (Eq a0 b0 A)).
+    have EC : erased_sort (Co (Eq a0 b0 A R0)).
     { inversion H1. apply erased_Co; eapply Typing_erased; eauto. }
     inversion GOOD.
     destruct (IHDefEq c) as [Ac h1]; auto.
@@ -1284,17 +1283,17 @@ Proof.
       * apply multipar_CAbs_exists; auto.
         apply (lc_a_UCAbs_exists c); try constructor; apply erased_lc; auto.
         eapply multipar_context_independent; eauto.
-  - intros G D a1 b1 B a b A d H p H0 H1.
+  - intros G D a1 b1 B R' a b A R d H p H0 H1.
     apply join_capp; auto.
-  - intros G D B1 B2 A1 A2 A A1' A2' A' H0 IHDefEq hi1 IHDefEq2 hi0 IHDefEq3 GOOD.
+  - intros G D B1 B2 R0 A1 A2 A R A1' A2' A' R' H0 IHDefEq hi1 IHDefEq2 hi0 IHDefEq3 GOOD.
     destruct IHDefEq as [Ac h0]; eauto.
     split_hyp.
     inversion GOOD.
     match goal with
-      [ H1 : erased_tm (a_CPi (Eq A1 A2 A) B1),
-        H2 : erased_tm (a_CPi (Eq A1' A2' A') B2),
-        H3 :  multipar G D (a_CPi (Eq A1 A2 A) B1) Ac,
-        H4 : multipar G D (a_CPi (Eq A1' A2' A') B2) Ac |- _ ] =>
+      [ H1 : erased_tm (a_CPi (Eq A1 A2 A R) B1),
+        H2 : erased_tm (a_CPi (Eq A1' A2' A' R') B2),
+        H3 :  multipar G D (a_CPi (Eq A1 A2 A R) B1) Ac,
+        H4 : multipar G D (a_CPi (Eq A1' A2' A' R') B2) Ac |- _ ] =>
       pose K1 := multipar_CPi H3 eq_refl;
       destruct K1 as [B1' [B2' [B3' [Bc' h0]]]];
       subst;
@@ -1340,36 +1339,62 @@ Proof.
         end.
       multipar_open_tm_wrt_co c B1.
     + multipar_open_tm_wrt_co c B2.
-  - intros G D A' B' a' A B a d H i H0 H1.
-    destruct (H0 H1 A B a A' B' a'); auto.
+  - intros G D A' B' a' R' A B a R d H i H0 H1.
+    destruct (H0 H1 A B a A' B' a' R R'); auto.
     move: (H H1) => h0.
     split_hyp.
     have h1 : joins G D A' B; eauto.
     apply join_transitive with (b := A); eauto.
     apply join_symmetry; auto.
     apply join_transitive with (b := B); eauto.
-  - intros G D A A' a b a' b' i H H0.
-    destruct (H H0 a b A a' b' A'); auto.
+  - intros G D A A' R a b a' b' i H H0.
+    destruct (H H0 a b A a' b' A' R R); auto.
     destruct H2; auto.
     Unshelve. all: auto.
+Admitted.
+
+Lemma consist_Pi_rEq : forall T1 T2, consistent T1 T2 ->
+               forall rho A1 A2 R1 R2 B1 B2,
+               lc_tm A1 -> lc_tm (a_Pi rho A1 R1 B1) ->
+               lc_tm A2 -> lc_tm (a_Pi rho A2 R2 B2) ->
+               T1 = a_Pi rho A1 R1 B1 -> T2 = a_Pi rho A2 R2 B2 ->
+               R1 = R2.
+Proof. intros T1 T2 H. induction H; intros.
+         - inversion H3.
+         - inversion H7. inversion H8. subst. auto.
+         - inversion H7.
+         - subst. assert False. apply H0. eauto. inversion H5.
+         - subst. assert False. apply H0. eauto. inversion H5.
 Qed.
 
+Lemma defEq_Pi_rEq : forall rho A1 A2 R1 R2 B1 B2 R' G D,
+             Good G D ->
+             DefEq G D (a_Pi rho A1 R1 B1) (a_Pi rho A2 R2 B2) a_Star R'
+             -> R1 = R2.
+Proof. intros. assert (H' := H0).
+       apply lc_mutual in H0.
+       inversion H0 as [H1 [H2 _]].
+       eapply consist_Pi_rEq. eapply join_consistent.
+       eapply consistent_mutual; eauto. inversion H1.
+       apply H5. apply H1. inversion H2. apply H5. 
+       apply H2. auto. auto.
+Qed.
 
-Lemma consistent_defeq: forall S D A B T,   DefEq S D A B T -> Good S D -> joins S D A B.
+Lemma consistent_defeq: forall S D A B T R,   DefEq S D A B T R -> Good S D -> joins S D A B.
 Proof.
   apply consistent_mutual.
 Qed.
 
 (* ------------------------------------------------------- *)
 
-Lemma no_aAbs : forall G rho A' a A, Typing G (a_Abs rho A' a) A -> False.
+Lemma no_aAbs : forall G rho A' a A R R', Typing G (a_Abs rho A' R' a) A R -> False.
 Proof.
-  intros. dependent induction H. by apply: IHTyping1.
+  intros. dependent induction H. by apply: IHTyping. by apply: IHTyping1.
 Qed.
 
-Lemma no_aCAbs : forall G A' a A, Typing G (a_CAbs A' a) A -> False.
+Lemma no_aCAbs : forall G A' a A R, Typing G (a_CAbs A' a) A R -> False.
 Proof.
-  intros. dependent induction H; by apply: IHTyping1.
+  intros. dependent induction H. by apply: IHTyping. by apply: IHTyping1.
 Qed.
 
 
@@ -1395,7 +1420,7 @@ Qed.
 
 
 Definition irrelevant G D (a : tm) :=
-  (forall x A, binds x (Tm A) G -> x `notin` fv_tm a) /\ Good G D.
+  (forall x A R, binds x (Tm A R) G -> x `notin` fv_tm a) /\ Good G D.
 
 Lemma irrelevant_Good : forall G D a, irrelevant G D a -> Good G D.
 intros. inversion H.
@@ -1411,7 +1436,7 @@ Ltac impossible_defeq :=
   let VT := fresh in
   let VT2 := fresh in
   match goal with
-  | [ H : DefEq ?G (dom ?G) ?B ?A ?C |- _ ] =>
+  | [ H : DefEq ?G (dom ?G) ?B ?A ?C ?R |- _ ] =>
     pose h0:= H; clearbody h0;
     apply consistent_defeq in h0; eauto;
     [apply join_consistent in h0;
@@ -1423,13 +1448,13 @@ Ltac impossible_defeq :=
   end.
 
 
-Lemma canonical_forms_Star : forall G a, irrelevant G (dom G) a ->
-    Typing G a a_Star -> Value a -> value_type a.
+Lemma canonical_forms_Star : forall G a R, irrelevant G (dom G) a ->
+    Typing G a a_Star R -> Value a -> value_type a.
 Proof.
-  intros G a IR H V. induction V; auto.
+  intros G a R IR H V. induction V; auto.
   - subst. assert False. eapply no_aAbs. eauto 2. done.
   - subst. apply invert_a_UAbs in H; eauto.
-    destruct H as [A1 [B2 [H _]]].
+    destruct H as [A1 [B2 [R0 [H _]]]].
     impossible_defeq.
   - subst. apply invert_a_UAbs in H; eauto.
     destruct H as (A1 & A2 & DE & TA1 & TA2).
@@ -1437,25 +1462,25 @@ Proof.
   - subst. assert False. eapply  no_aAbs. eauto 2. done.
   - subst.  assert False. eapply no_aCAbs. eauto 2. done.
   - subst. apply invert_a_UCAbs in H; eauto.
-    destruct H as [a0 [b [T [B1 [_ [H _]]]]]].
+    destruct H as [a0 [b [T [R1 [B1 [R2 [_ [H _]]]]]]]].
     impossible_defeq.
 Qed.
 
 
 
-Lemma DefEq_Star: forall A G D, Good G D -> value_type A -> DefEq G D A a_Star a_Star -> A = a_Star.
+Lemma DefEq_Star: forall A G D R, Good G D -> value_type A -> DefEq G D A a_Star a_Star R -> A = a_Star.
 Proof.
-  intros A G D Good H0 H.
+  intros A G D R Good H0 H.
   apply consistent_defeq in H; eauto.
   apply join_consistent in H.
   inversion H;  eauto; subst; try done.
 Qed.
 
-Lemma canonical_forms_Pi : forall G rho a A B, irrelevant G (dom G) a ->
-    Typing G a (a_Pi rho A B) -> Value a ->
+Lemma canonical_forms_Pi : forall G rho a A R B R', irrelevant G (dom G) a ->
+    Typing G a (a_Pi rho A R B) R' -> Value a ->
     (exists a1, a = a_UAbs rho a1).
 Proof.
-  intros G rho a A B IR H H0.
+  intros G rho a A R B R' IR H H0.
   inversion H0; subst; eauto.
   - apply invert_a_Star in H; eauto.
     impossible_defeq.
@@ -1467,23 +1492,23 @@ Proof.
     impossible_defeq.
   - assert False. eapply no_aAbs. eauto 2. done.
   - eapply invert_a_UAbs in H; eauto.
-    destruct H as (A1 & A2 & H & _); eauto.
+    destruct H as (A1 & A2 & R0 & H & _); eauto.
     impossible_defeq.
   - eapply invert_a_UAbs in H; eauto.
-    destruct H as (A1 & B1 & H & _); eauto.
+    destruct H as (A1 & B1 & R0 & H & _); eauto.
     impossible_defeq.
   - assert False. eapply no_aAbs. eauto 2. done.
   - assert False. eapply no_aCAbs. eauto 2. done.
   - eapply invert_a_UCAbs in H; eauto.
-    destruct H as [a [b [T [B1 [_ [H _]]]]]]; eauto.
+    destruct H as [a [b [T [R1 [B1 [_ [_ [H _]]]]]]]]; eauto.
     impossible_defeq.
 Qed.
 
-Lemma canonical_forms_CPi : forall G a phi B, irrelevant G (dom G) a ->
-    Typing G a (a_CPi phi B) -> Value a ->
+Lemma canonical_forms_CPi : forall G a phi B R, irrelevant G (dom G) a ->
+    Typing G a (a_CPi phi B) R -> Value a ->
     (exists a1, a = a_UCAbs a1).
 Proof.
-  intros G a phi B IR H H0.
+  intros G a phi B R IR H H0.
   inversion H0; subst; eauto.
   - apply invert_a_Star in H; eauto.
     impossible_defeq.
@@ -1495,10 +1520,10 @@ Proof.
     impossible_defeq.
   - assert False. eapply no_aAbs. eauto 2. done.
   - eapply invert_a_UAbs in H; eauto.
-    destruct H as [A1 [A2 [H _]]]; eauto.
+    destruct H as [A1 [A2 [R' [H _]]]]; eauto.
     impossible_defeq.
   - eapply invert_a_UAbs in H; eauto.
-    destruct H as [A1 [A2 [H _]]]; eauto.
+    destruct H as [A1 [A2 [R' [H _]]]]; eauto.
     impossible_defeq.
   - assert False. eapply no_aAbs. eauto 2. done.
   - assert False. eapply no_aCAbs. eauto 2. done.
@@ -1517,7 +1542,7 @@ Ltac show_irrelevant IR :=
         let h1 := fresh in
         unfold irrelevant in *;
         move: IR => [h0 h1]; split; auto;
-        intros x A0 B0;  apply h0 in B0; simpl in B0; fsetdec.
+        intros x A0 R0 B0;  apply h0 in B0; simpl in B0; fsetdec.
 
 Lemma notin_sub : forall x a b, x `notin` a -> b [<=] a -> x `notin` b.
   intros. fsetdec.
@@ -1530,7 +1555,7 @@ Qed.
    which is a subrelation of the Par relation.
 *)
 
-Lemma progress : forall G a A, Typing G a A ->
+Lemma progress : forall G a A R, Typing G a A R ->
                           irrelevant G (dom G) a ->
                           Value a \/ exists a', reduction_in_one a a'.
   induction 1; intros IR; subst; eauto; try done.
@@ -1554,19 +1579,19 @@ Lemma progress : forall G a A, Typing G a A ->
     apply (Typing_lc (H x h0)); eauto.
     + pick fresh x.
       assert (x `notin` L). auto.
-      move: (H2 x H3) => h0.
+      move: (H2 x H4) => h0.
       inversion h0. subst.
-      destruct (H0 x H3) as [V | [a' R]].
-      { move: (H x H3) => h1.
+      destruct (H0 x H4) as [V | [a' T]].
+      { move: (H x H4) => h1.
       unfold irrelevant in *.
       destruct IR as [h2 h3].
-      have ctx: (Ctx ([(x, Tm A)] ++ G)) by eauto.
+      have ctx: (Ctx ([(x, Tm A R)] ++ G)) by eauto.
       move: (Ctx_uniq ctx) => u. inversion u. subst.
-      split. intros x0 A0 b0.
+      split. intros x0 A0 R0 b0.
       apply binds_cons_uniq_1 in b0. destruct b0.
       ++ split_hyp. subst. auto.
       ++ split_hyp.
-         move: (h2 _ _ H5) => fr. simpl in fr.
+         move: (h2 _ _ _ H6) => fr. simpl in fr.
          eapply notin_sub; [idtac|eapply fv_tm_tm_tm_open_tm_wrt_tm_upper].
          simpl.
          fsetdec.
