src/FcEtt/ett_ind.v
@@ -732,3 +732,4 @@ Proof.
 Qed.
 
 Hint Rewrite tm_subst_cast.
+
